Monus defined

HOL-ETCS/Monus.thy
@@ -1,20 +1,131 @@
 theory Monus
-  imports Add
+  imports Add Inequality
 begin
 
 definition monus1 :: "cfunc" 
-  where "monus1 = (THE u. u : \<nat>\<^sub>c \<rightarrow> \<nat>\<^sub>c\<^bsup>\<nat>\<^sub>c\<^esup> \<and> u \<circ>\<^sub>c zero = ((left_coproj \<nat>\<^sub>c \<one>) \<circ>\<^sub>c (left_cart_proj \<nat>\<^sub>c \<one>))\<^sup>\<sharp> \<and> 
+  where "monus1 = (THE u. u : \<nat>\<^sub>c \<rightarrow> \<nat>\<^sub>c\<^bsup>\<nat>\<^sub>c\<^esup> \<and> 
+  u \<circ>\<^sub>c zero = (left_cart_proj \<nat>\<^sub>c \<one>)\<^sup>\<sharp> \<and> 
   u \<circ>\<^sub>c successor = predecessor\<^bsup>\<nat>\<^sub>c\<^esup>\<^sub>f \<circ>\<^sub>c u)"
 
+lemma monus1_property: "monus1 : \<nat>\<^sub>c \<rightarrow> \<nat>\<^sub>c\<^bsup>\<nat>\<^sub>c\<^esup> \<and> 
+  monus1 \<circ>\<^sub>c zero = (left_cart_proj \<nat>\<^sub>c \<one>)\<^sup>\<sharp> \<and> 
+  monus1 \<circ>\<^sub>c successor = predecessor\<^bsup>\<nat>\<^sub>c\<^esup>\<^sub>f \<circ>\<^sub>c monus1"
+  unfolding monus1_def
+  by (rule theI', typecheck_cfuncs, smt (verit, best) natural_number_object_property2)
+  
+lemma monus1_type[type_rule]: "monus1: \<nat>\<^sub>c \<rightarrow> \<nat>\<^sub>c\<^bsup>\<nat>\<^sub>c\<^esup>"
+  by (simp add: monus1_property)
 
-
+lemma monus1_0_eq: "monus1 \<circ>\<^sub>c zero = left_cart_proj \<nat>\<^sub>c \<one>\<^sup>\<sharp>"
+  by (simp add: monus1_property)
+  
+lemma monus1_succ_eq: "monus1 \<circ>\<^sub>c successor = predecessor\<^bsup>\<nat>\<^sub>c\<^esup>\<^sub>f \<circ>\<^sub>c monus1"
+  by (simp add: monus1_property)
 
 definition monus2 :: "cfunc" 
-  where "monus2   = eval_func  \<nat>\<^sub>c \<nat>\<^sub>c \<circ>\<^sub>c (id \<nat>\<^sub>c \<times>\<^sub>f monus1)"
+  where "monus2   = eval_func \<nat>\<^sub>c \<nat>\<^sub>c \<circ>\<^sub>c (id \<nat>\<^sub>c \<times>\<^sub>f monus1)"
 
+lemma monus2[type_rule]: "monus2: \<nat>\<^sub>c \<times>\<^sub>c \<nat>\<^sub>c \<rightarrow>  \<nat>\<^sub>c"
+  unfolding monus2_def
+  using flat_type inv_transpose_func_def3 monus1_type by force
+
+lemma monus2_apply:
+  assumes "m : X \<rightarrow> \<nat>\<^sub>c" "n : X \<rightarrow> \<nat>\<^sub>c"
+  shows "monus2 \<circ>\<^sub>c \<langle>m, n\<rangle> = eval_func  \<nat>\<^sub>c \<nat>\<^sub>c \<circ>\<^sub>c \<langle>m, monus1 \<circ>\<^sub>c n\<rangle>"
+  unfolding monus2_def using assms 
+  by (etcs_assocr, typecheck_cfuncs, smt cfunc_cross_prod_comp_cfunc_prod id_left_unit2)
 
 definition monus :: "cfunc \<Rightarrow> cfunc \<Rightarrow> cfunc" (infixl "\<midarrow>\<^sub>\<nat>" 65)
   where "m \<midarrow>\<^sub>\<nat> n = monus2 \<circ>\<^sub>c \<langle>m, n\<rangle>"
+
+lemma  monus_type[type_rule]:
+  assumes "m : X \<rightarrow> \<nat>\<^sub>c" "n : X \<rightarrow> \<nat>\<^sub>c"
+  shows "m \<midarrow>\<^sub>\<nat> n : X \<rightarrow> \<nat>\<^sub>c"
+  unfolding monus_def using assms by typecheck_cfuncs
+
+lemma monus_def2:
+  assumes "m \<in>\<^sub>c \<nat>\<^sub>c" "n \<in>\<^sub>c \<nat>\<^sub>c"
+  shows "m \<midarrow>\<^sub>\<nat> n = eval_func  \<nat>\<^sub>c \<nat>\<^sub>c \<circ>\<^sub>c \<langle>m, monus1 \<circ>\<^sub>c n\<rangle>"
+  unfolding monus_def using assms by (typecheck_cfuncs, simp add: monus2_apply)
+
+lemma monus_zero:
+  assumes n_type[type_rule]: "n \<in>\<^sub>c \<nat>\<^sub>c"
+  shows "n \<midarrow>\<^sub>\<nat> zero = n"
+proof - 
+  have "n \<midarrow>\<^sub>\<nat> zero = eval_func  \<nat>\<^sub>c \<nat>\<^sub>c \<circ>\<^sub>c \<langle>n, left_cart_proj \<nat>\<^sub>c \<one>\<^sup>\<sharp>\<rangle>"
+    using monus1_0_eq monus_def2 by (typecheck_cfuncs, presburger)
+  also have "... = eval_func  \<nat>\<^sub>c \<nat>\<^sub>c \<circ>\<^sub>c \<langle>id \<nat>\<^sub>c \<circ>\<^sub>c n, left_cart_proj \<nat>\<^sub>c \<one>\<^sup>\<sharp> \<circ>\<^sub>c id \<one>\<rangle>"
+    using assms by (typecheck_cfuncs, simp add: id_left_unit2 id_right_unit2)
+  also have "... = eval_func  \<nat>\<^sub>c \<nat>\<^sub>c \<circ>\<^sub>c (id \<nat>\<^sub>c \<times>\<^sub>f  left_cart_proj \<nat>\<^sub>c \<one>\<^sup>\<sharp>) \<circ>\<^sub>c \<langle>n, id \<one>\<rangle>"
+    using assms by (typecheck_cfuncs, simp add: cfunc_cross_prod_comp_cfunc_prod)
+  also have "... =  left_cart_proj \<nat>\<^sub>c \<one> \<circ>\<^sub>c \<langle>n,id \<one>\<rangle>"
+    using assms by (typecheck_cfuncs, simp add: comp_associative2 transpose_func_def)
+  also have "... = n"
+    using assms id_type left_cart_proj_cfunc_prod by blast
+  then show "n \<midarrow>\<^sub>\<nat> zero = n"
+    using calculation by auto
+qed
+
+(*Restate as "smallest such solution"*)
+lemma monus_def3: 
+  assumes m_type[type_rule]: "m \<in>\<^sub>c \<nat>\<^sub>c" and n_type[type_rule]: "n \<in>\<^sub>c \<nat>\<^sub>c"
+  shows "m \<le>\<^sub>\<nat> n +\<^sub>\<nat> (n \<midarrow>\<^sub>\<nat> m)"
+  apply typecheck_cfuncs
+
+lemma predecessor_nonzero:
+  assumes n_type[type_rule]: "n \<in>\<^sub>c \<nat>\<^sub>c"
+  assumes nonzero: "n \<noteq> zero"
+  shows "predecessor \<circ>\<^sub>c n = n \<midarrow>\<^sub>\<nat> (successor \<circ>\<^sub>c zero)"
+  sorry
+(*
+proof - 
+  obtain m where m_type[type_rule]: "m \<in>\<^sub>c \<nat>\<^sub>c" and m_def: "n = successor \<circ>\<^sub>c m"
+    using n_type nonzero nonzero_is_succ by auto
+  have "predecessor \<circ>\<^sub>c n = m"
+    using comp_associative2 id_left_unit2 m_def predecessor_successor successor_type by (typecheck_cfuncs, force)
+  also have "... = n \<midarrow>\<^sub>\<nat> (successor \<circ>\<^sub>c zero)"
+    apply typecheck_cfuncs
+    oops
+*)
+
+lemma zero_monus:
+  assumes n_type[type_rule]: "n \<in>\<^sub>c \<nat>\<^sub>c"
+  shows "zero \<midarrow>\<^sub>\<nat> n = zero"
+proof - 
+  have "(eq_pred \<nat>\<^sub>c \<circ>\<^sub>c \<langle>monus2 \<circ>\<^sub>c \<langle>zero \<circ>\<^sub>c \<beta>\<^bsub>\<nat>\<^sub>c\<^esub>, id \<nat>\<^sub>c\<rangle>, zero \<circ>\<^sub>c \<beta>\<^bsub>\<nat>\<^sub>c\<^esub>\<rangle>) \<circ>\<^sub>c n = \<t>"
+  proof(etcs_rule nat_induction)
+    show "(eq_pred \<nat>\<^sub>c \<circ>\<^sub>c \<langle>monus2 \<circ>\<^sub>c \<langle>zero \<circ>\<^sub>c \<beta>\<^bsub>\<nat>\<^sub>c\<^esub>,id\<^sub>c \<nat>\<^sub>c\<rangle>,zero \<circ>\<^sub>c \<beta>\<^bsub>\<nat>\<^sub>c\<^esub>\<rangle>) \<circ>\<^sub>c zero = \<t>"
+      by (typecheck_cfuncs, smt (z3) cart_prod_extract_right cfunc_prod_comp comp_associative2
+          eq_pred_iff_eq_conv2 monus_def monus_zero terminal_func_comp zero_betaN_type)
+  next
+    fix m 
+    assume m_type[type_rule]: "m \<in>\<^sub>c \<nat>\<^sub>c"
+    assume eq_pred_ind_hyp: "(eq_pred \<nat>\<^sub>c \<circ>\<^sub>c \<langle>monus2 \<circ>\<^sub>c \<langle>zero \<circ>\<^sub>c \<beta>\<^bsub>\<nat>\<^sub>c\<^esub>,id\<^sub>c \<nat>\<^sub>c\<rangle>,zero \<circ>\<^sub>c \<beta>\<^bsub>\<nat>\<^sub>c\<^esub>\<rangle>) \<circ>\<^sub>c n = \<t>"
+    have induction_hypothesis: "monus2 \<circ>\<^sub>c \<langle>zero, n\<rangle> = zero"
+    proof - 
+      have "\<t> = eq_pred \<nat>\<^sub>c \<circ>\<^sub>c \<langle>monus2 \<circ>\<^sub>c \<langle>zero \<circ>\<^sub>c \<beta>\<^bsub>\<nat>\<^sub>c\<^esub>, id\<^sub>c \<nat>\<^sub>c\<rangle>, zero \<circ>\<^sub>c \<beta>\<^bsub>\<nat>\<^sub>c\<^esub>\<rangle> \<circ>\<^sub>c n"
+        using eq_pred_ind_hyp comp_associative2 by (typecheck_cfuncs, force)
+      also have "... = eq_pred \<nat>\<^sub>c \<circ>\<^sub>c \<langle>monus2 \<circ>\<^sub>c \<langle>zero, n\<rangle>, zero\<rangle>"
+        by (typecheck_cfuncs, smt (verit, best) cart_prod_extract_right cfunc_prod_comp comp_associative2 id_right_unit2 terminal_func_comp_elem)
+      then show ?thesis
+        by (typecheck_cfuncs, simp add: calculation eq_pred_iff_eq)
+    qed
+    have induction_conclusion: "monus2 \<circ>\<^sub>c \<langle>zero, successor \<circ>\<^sub>c n\<rangle> = zero"
+    proof - 
+      oops
+
+
+
+
+(*
+lemma monus_succ_is_pred_monus:
+  assumes m_type[type_rule]: "m \<in>\<^sub>c \<nat>\<^sub>c" and n_type[type_rule]: "n \<in>\<^sub>c \<nat>\<^sub>c"
+  shows "m \<midarrow>\<^sub>\<nat> (successor \<circ>\<^sub>c n) = predecessor \<circ>\<^sub>c (m \<midarrow>\<^sub>\<nat> n)"
+proof(cases "m = zero")
+  show "m = zero \<Longrightarrow> m \<midarrow>\<^sub>\<nat> (successor \<circ>\<^sub>c n) = predecessor \<circ>\<^sub>c m \<midarrow>\<^sub>\<nat> n"
+    apply typecheck_cfuncs
+*)
+
 
 
 end
